work in progress with frameable WPs

pulse/examples/steel_wip/ParDivWP.fst
@@ -44,6 +44,32 @@ let commutative #a (f: a -> a -> a) =
 let is_unit #a (x:a) (f:a -> a -> a) =
   forall y. f x y == y /\ f y x == y
 
+let split_idem #r #s (split:r -> s -> s & s) =
+  forall r s. 
+    let s0, _ = split r s in
+    let s0', _ = split r s0 in
+    s0 == s0'
+
+let split_join #r #s (split:r -> s -> s & s) (join: s & s -> s) = 
+    forall (r0:r) (s:s). 
+      join (split r0 s) == s
+
+let join_split #r #s (split:r -> s -> s & s) (join: s & s -> s) (star:r -> r -> r) (inv: r -> s -> prop) = 
+    forall (r0 r1:r) (s0 s1:s). 
+       inv (r0 `star` r1) (join (s0, s1)) /\
+       inv r0 s0 /\
+       inv r1 s1 ==>
+       fst (split r0 (join (s0, s1))) == s0
+
+let split_star #r #s (split:r -> s -> s & s) (star: r -> r -> r) (inv:r -> s -> prop) = 
+    forall (r0 r1:r) (s:s). 
+      inv (r0 `star` r1) s ==> (
+      let s0, s = split r0 s in
+      inv r0 s0 /\
+      inv r1 s)
+
+let affine #r #s (star:r -> r -> r) (inv: r -> s -> prop) =
+  forall r0 r1 s. inv (r0 `star` r1) s ==> inv r0 s
 
 (**
  * In addition to being a commutative monoid over the carrier [r]
@@ -51,85 +77,223 @@ let is_unit #a (x:a) (f:a -> a -> a) =
  * as a predicate on states [s]
  *)
 noeq
-type comm_monoid (s:Type) = {
+type st = {
+  s:Type;
   r:Type;
   emp: r;
   star: r -> r -> r;
   interp: r -> s -> prop;
-  laws: squash (associative star /\ commutative star /\ is_unit emp star)
+  split: r -> s -> s & s;
+  join: s & s -> s;
+  laws: squash (
+    associative star /\
+    commutative star /\
+    is_unit emp star /\
+    split_idem split /\
+    split_join split join /\
+    join_split split join star interp /\
+    split_star split star interp /\
+    affine star interp)
 }
 
 (** [post a c] is a postcondition on [a]-typed result *)
-let post #s a (c:comm_monoid s) = a -> c.r
+let post (st:st) (a:Type) = a -> st.r
 
-(** [action c s]: atomic actions are, intuitively, single steps of
- *  computations interpreted as a [s -> a & s].
- *  However, we augment them with two features:
- *   1. they have pre-condition [pre] and post-condition [post]
- *   2. their type guarantees that they are frameable
- *  Thanks to Matt Parkinson for suggesting to set up atomic actions
- *  this way.
- *  Also see: https://www.microsoft.com/en-us/research/wp-content/uploads/2016/02/views.pdf
- *)
 noeq
-type action #s (c:comm_monoid s) (a:Type) = {
-   pre: c.r;
-   post: a -> c.r;
-   sem: (frame:c.r ->
-         s0:s{c.interp (c.star pre frame) s0} ->
-         (x:a & s1:s{c.interp (post x `c.star` frame) s1}));
-}
+type action (st:st) (a:Type) = {
+   pre: st.r;
+   post: a -> st.r;
+   sem: (s0:st.s{st.interp pre s0}) -> (a & st.s);
+   action_ok: squash (
+     (forall (frame:st.r) (s0:st.s).
+       st.interp (pre `st.star` frame) s0 ==>
+       (let x, s1 = sem s0 in
+        st.interp (post x `st.star` frame) s1)) /\
+     (forall (frame:st.r) s. 
+       st.interp (pre `st.star` frame) s ==>
+       (let s_pre, s_frame = st.split pre s in
+        let x, s1 = sem s_pre in
+        sem s == (x, st.join (s1, s_frame)))))
+}    
 
-let rs (#s:Type) (#c:comm_monoid s) (pre:c.r) = state:s{c.interp pre state}
-let wp_post (#s:Type) (#c:comm_monoid s) (a:Type) (post:post a c) = (x:a -> rs (post x) -> prop)
-let wp_pre (#s:Type) (#c:comm_monoid s) (pre:c.r) = rs pre -> prop
-let wp (#s:Type) (#c:comm_monoid s) (pre:c.r) (a:Type) (post:post a c) = wp_post a post -> wp_pre pre
-let triv_wp (#s:Type) (#c:comm_monoid s) 
-            (pre:c.r)
+let rs (#st:st) (pre:st.r) = state:st.s{st.interp pre state}
+
+let rs_prop' (#st:st) (pre:st.r) = rs pre -> prop
+
+// only depends on the `pre` footprint of s
+let rs_prop  (#st:st) (pre:st.r) = 
+  p: rs_prop' pre {
+    forall (s:st.s) (frame:st.r). 
+      st.interp (pre `st.star` frame) s ==>
+      (p s <==> p (fst (st.split pre s)))
+  }
+
+let wp_post (#st:st) (a:Type) (post:post st a) = x:a -> rs_prop (post x)
+let wp_pre (#st:st) (pre:st.r) = rs_prop pre
+let wp (#st:st) (pre:st.r) (a:Type) (post:post st a) = wp_post a post -> wp_pre pre
+
+let triv_wp (#st:st)
+            (pre:st.r)
             (a:Type) 
-            (post:post a c)
+            (post:post st a)
   : wp pre a post
-  = fun (k:wp_post a post) (s0:rs pre) -> forall (x:a) (s1:rs (post x)). k x s1
-let return_wp (#s:Type) (#c:comm_monoid s) (#a:Type) (x:a) (post: post a c)
+  = fun (k:wp_post a post) -> 
+      let pre : rs_prop' pre =
+        fun (s0:rs pre) ->
+          forall (x:a) (s1:rs (post x)). k x s1
+      in
+      pre
+
+let return_wp (#st:st) (#a:Type) (x:a) (post: post st a)
   : wp (post x) a post
-  = fun k s0 -> k x s0 
-let bind_wp (#s:Type) (#c:comm_monoid s)
-            (#pre_a:c.r) (#a:Type) (#post_a:post a c)
-            (#b:Type) (#post_b:post b c)
+  = fun (k:wp_post a post) ->
+      let pre : rs_prop' (post x) =
+        fun s0 -> k x s0 
+      in
+      pre
+
+let bind_wp (#st:st)
+            (#pre_a:st.r) (#a:Type) (#post_a:post st a)
+            (#b:Type) (#post_b:post st b)
             (f:wp pre_a a post_a)
             (g: (x:a -> wp (post_a x) b post_b))
   : wp pre_a b post_b
   = fun k -> f (fun x -> g x k)
- 
-let bind_action #s (#c:comm_monoid s) #a #b 
-                (f:action c b)
-                (#post_g:post a c)
+
+let wp_action (#st:st) #b (f:action st b)
+  : wp f.pre b f.post
+  = fun (k:wp_post b f.post) -> 
+      let pre : rs_prop' f.pre =
+        fun (s0:rs f.pre) -> 
+         assert (st.interp (f.pre `st.star` st.emp) s0);
+         let s0, s_frame = st.split f.pre s0 in
+         let x, s0' = f.sem s0 in
+         let s1 = st.join (s0', s_frame) in
+         assert (st.interp (f.post x `st.star` st.emp) s1);
+         k x s1
+     in
+     pre
+     // let aux0 (s:st.s) (frame:st.r)
+     //   : Lemma 
+     //     (requires (st.interp (f.pre `st.star` frame) s /\ pre s))
+     //     (ensures (pre (fst (st.split f.pre s))))
+     //     [SMTPat (st.interp (f.pre `st.star` frame) s)]
+     //   = ()
+     // in
+     // let aux1 (s:st.s) (frame:st.r)
+     //   : Lemma 
+     //     (requires (st.interp (f.pre `st.star` frame) s /\ (pre (fst (st.split f.pre s)))))
+     //     (ensures (pre s))
+     //     [SMTPat (st.interp (f.pre `st.star` frame) s)]
+     //   = let s0, s_frame = st.split f.pre s in
+     //     let s0', s_frame' = st.split f.pre s0 in
+     //     assert (s0 == s0');
+     //     let x, s0'' = f.sem s0' in
+     //     let s1' = st.join (s0'', s_frame') in
+     //     let kk : rs_prop (f.post x) = k x in         
+     //     assert (kk s1');
+     //     let s1 = st.join (s0'', s_frame) in
+     //     assert (kk (fst (st.split (f.post x) s1')));
+     //     assert (fst (st.split (f.post x) s1) ==
+     //             fst (st.split (f.post x) s1'));
+     //     assert (kk s1)
+     // in
+     // pre
+
+let bind_action (#st:st) #a #b 
+                (f:action st b)
+                (#post_g:post st a)
                 (wp_g:(x:b -> wp (f.post x) a post_g))
    : wp f.pre a post_g
-   = fun k s0 -> 
-       let (| x, s1 |) = f.sem c.emp s0 in
-       wp_g x k s1
+   = bind_wp (wp_action f) wp_g
 
-let wp_par #s (#c:comm_monoid s) (#pre: c.r)
-             #a0 (pre0:_) (post0: post a0 c) (wp0: wp pre0 a0 post0)
-             #a1 (pre1:_) (post1: post a1 c) (wp1: wp pre1 a1 post1)
-   : wp (pre0 `c.star` pre1) (a0 & a1) (fun (x0, x1) -> post0 x0 `c.star` post1 x1)
-   = fun k s -> 
-      let s0, s1, frame = split s pre0 pre1 in
-      as_requires wp0 s0 /\
-      as_requires wp1 s1 /\      
-      (forall x0 s0' x1 s1'. 
-        joinable s0' s1' frame /\
-        as_ensures wp0 s0 x0 s0' /\
-        as_ensures wp1 s1 x1 s1' ==>
-        k (x0, x1) (join s0' s1' frame))
+assume
+val as_requires (#st:_) (#aL:Type) (#preL:st.r) (#postL: post st aL) (wpL: wp preL aL postL)
+  : rs_prop preL
 
-let bind_par #s (#c:comm_monoid s) (#pre: c.r)
-             #a0 (post0: post a0 c)
-             #a1 (post1: post a1 c)   
-             #a  #post (wp_a:(x0:a0 -> x1:a1 -> wp (post0 x0 `c.star` post1 x1) a post))
-   : wp pre a post
-   = (fun k s0 -> forall (x0:a0) (x1:a1) (s1:rs (c.star (post0 x0) (post1 x1))). wp_a x0 x1 k s1)
+assume
+val as_ensures (#st:_) (#aL:Type) (#preL:st.r) (#postL: post st aL) (wpL: wp preL aL postL) (sL:rs preL)
+  : wp_post aL postL
+
+module C = FStar.Classical
+let wp_par (#st:st)
+           #aL (preL:st.r) (postL: post st aL) (wpL: wp preL aL postL)
+           #aR (preR:st.r) (postR: post st aR) (wpR: wp preR aR postR)
+   : wp (preL `st.star` preR) 
+        (aL & aR)
+        (fun (xL, xR) -> postL xL `st.star` postR xR)
+   = fun (k:wp_post (aL & aR) (fun (xL, xR) -> postL xL `st.star` postR xR)) -> 
+       let post xL sL' xR sR' rest : prop =
+           let s1 = st.join (sL', st.join (sR', rest)) in
+           // as_ensures wpL sL xL sL' /\
+           // as_ensures wpR sR xR sR' /\
+           st.interp (postL xL) sL' /\
+           st.interp (postR xR) sR' /\             
+           st.interp (postL xL `st.star` postR xR) s1 ==>
+           k (xL, xR) s1
+       in
+       let pre : rs_prop' (preL `st.star` preR) =
+         fun (s0:rs (preL `st.star` preR)) -> 
+           let sL, rest = st.split preL s0 in
+           let sR, rest = st.split preR rest in
+           assert (st.interp preL sL);
+           assert (st.interp preR sR);
+           as_requires wpL sL /\
+           as_requires wpR sR /\           
+           (forall xL sL' xR sR'. post xL sL' xR sR' rest)
+       in
+       let aux0 (s:st.s)
+         : Lemma 
+           (requires (st.interp (preL `st.star` preR) s /\ pre s))
+           (ensures (pre (fst (st.split (preL `st.star` preR) s))))
+           [SMTPat (st.interp (preL `st.star` preR) s)]
+         = admit()
+       in
+       let aux1 (s:st.s)
+         : Lemma 
+           (requires (st.interp (preL `st.star` preR) s /\ 
+                     (pre (fst (st.split (preL `st.star` preR) s)))))
+           (ensures pre s)
+           [SMTPat (st.interp (preL `st.star` preR) s)]
+         = let sL, rest = st.split preL s in
+           let sR, rest = st.split preR rest in
+           
+           let s', _ = st.split (preL `st.star` preR) s in
+           let sL', rest' = st.split preL s' in
+           let sR', rest' = st.split preR rest' in
+           assume (sL == sL');
+           assume (sR == sR');
+           let aux xL sL'' xR sR''
+             : Lemma 
+               (requires
+                 post xL sL'' xR sR'' rest')
+               (ensures
+                 post xL sL'' xR sR'' rest)
+               [SMTPat (k (xL, xR) (st.join (sL'', st.join (sR'', rest))))]
+             = let s1' = st.join (sL'', st.join (sR'', rest')) in             
+               let s1 = st.join (sL'', st.join (sR'', rest)) in             
+               let aux ()
+                 : Lemma 
+                   (requires 
+                       (st.interp (postL xL) sL'' /\
+                        st.interp (postR xR) sR'' /\
+                        st.interp (postL xL `st.star` postR xR) s1))
+                   (ensures 
+                       k (xL, xR) s1)
+                   [SMTPat ()]
+                 = assume (st.interp (postL xL `st.star` postR xR) s1');
+                   assert (k (xL, xR) s1');
+                   assert (k (xL, xR) (fst (st.split (postL xL `st.star` postR xR) s1')));
+                   assume (fst (st.split (postL xL `st.star` postR xR) s1') ==
+                           fst (st.split (postL xL `st.star` postR xR) s1));
+                   assert (k (xL, xR) s1)
+               in
+               ()
+           in
+           ()
+       in
+       pre
+
              
 
 (** [m s c a pre post] :
@@ -272,150 +436,150 @@ let rec step #s #c (i:nat) #pre #a #post
                   j
         else admit()
         
-        let Step pre1' m1' state' j =
-                 step (i + 1) m1 (pre0 `c.star` frame) state in
-             Step (pre0 `c.star` pre1') (Par pre0 post0 m0 pre1' post1 m1' k) state' j
+//         let Step pre1' m1' state' j =
+//                  step (i + 1) m1 (pre0 `c.star` frame) state in
+//              Step (pre0 `c.star` pre1') (Par pre0 post0 m0 pre1' post1 m1' k) state' j
 
-// (**
-//  * [run i f state]: Top-level driver that repeatedly invokes [step]
-//  *
-//  * The type of [run] is the main theorem. It states that it is sound
-//  * to interpret the indices of `m` as a Hoare triple in a
-//  * partial-correctness semantics
-//  *
-//  *)
-// let rec run #s #c (i:nat) #pre #a #post (f:m s c a pre post) (state:s)
-//   : Div (a & s)
-//     (requires
-//       c.interp pre state)
-//     (ensures fun (x, state') ->
-//       c.interp (post x) state')
-//   = match f with
-//     | Ret x -> x, state
-//     | _ ->
-//       let Step pre' f' state' j = step i f c.emp state in
-//       run j f' state'
+// // (**
+// //  * [run i f state]: Top-level driver that repeatedly invokes [step]
+// //  *
+// //  * The type of [run] is the main theorem. It states that it is sound
+// //  * to interpret the indices of `m` as a Hoare triple in a
+// //  * partial-correctness semantics
+// //  *
+// //  *)
+// // let rec run #s #c (i:nat) #pre #a #post (f:m s c a pre post) (state:s)
+// //   : Div (a & s)
+// //     (requires
+// //       c.interp pre state)
+// //     (ensures fun (x, state') ->
+// //       c.interp (post x) state')
+// //   = match f with
+// //     | Ret x -> x, state
+// //     | _ ->
+// //       let Step pre' f' state' j = step i f c.emp state in
+// //       run j f' state'
 
-// ////////////////////////////////////////////////////////////////////////////////
-// //The rest of this module shows how this semantic can be packaged up as an
-// //effect in F*
-// ////////////////////////////////////////////////////////////////////////////////
+// // ////////////////////////////////////////////////////////////////////////////////
+// // //The rest of this module shows how this semantic can be packaged up as an
+// // //effect in F*
+// // ////////////////////////////////////////////////////////////////////////////////
 
-// (** [eff a pre post] : The representation-type for a layered effect
-//  *
-//  *   - Note, we'll probably have to add a thunk to make it work with
-//  *     the current implementation but that's a detail
-//  *)
-// let eff #s (#c:comm_monoid s) a (pre:c.r) (post: a -> c.r) =
-//   m s c a pre post
+// // (** [eff a pre post] : The representation-type for a layered effect
+// //  *
+// //  *   - Note, we'll probably have to add a thunk to make it work with
+// //  *     the current implementation but that's a detail
+// //  *)
+// // let eff #s (#c:comm_monoid s) a (pre:c.r) (post: a -> c.r) =
+// //   m s c a pre post
 
-// /// eff is a monad: we give a return and bind for it, though we don't
-// /// prove the monad laws
-
-
-// (** [return]: easy, just use Ret *)
-// let return #s (#c:comm_monoid s) #a (x:a) (post:a -> c.r)
-//   : eff a (post x) post
-//   = Ret x
-
-// (**
-//  * [bind]: sequential composition works by pushing `g` into the continuation
-//  * at each node, finally applying it at the terminal `Ret`
-//  *)
-// let rec bind #s (#c:comm_monoid s) #a #b (#p:c.r) (#q:a -> c.r) (#r:b -> c.r)
-//              (f:eff a p q)
-//              (g: (x:a -> eff b (q x) r))
-//   : Dv (eff b p r)
-//   = match f with
-//     | Ret x -> g x
-//     | Act act k ->
-//       Act act (fun x -> bind (k x) g)
-//     | Par pre0 post0 l
-//           pre1 post1 r
-//           k ->
-//       Par pre0 post0 l pre1 post1 r (fun x0 x1 -> bind (k x0 x1) g)
-
-// (**
-//  * [par]: Parallel composition
-//  * Works by just using the `Par` node and `Ret` as its continuation
-//  **)
-// let par #s (#c:comm_monoid s)
-//         #a0 #p0 #q0 (m0:eff a0 p0 q0)
-//         #a1 #p1 #q1 (m1:eff a1 p1 q1)
-//  : eff (a0 & a1) (p0 `c.star` p1) (fun (x0, x1) -> q0 x0 `c.star` q1 x1)
-//  = Par p0 q0 m0
-//        p1 q1 m1
-//        #_ #(fun (x0, x1) -> c.star (q0 x0) (q1 x1)) (fun x0 x1 -> Ret (x0, x1))
+// // /// eff is a monad: we give a return and bind for it, though we don't
+// // /// prove the monad laws
 
 
-// /// Now for an instantiation of the state with a heap
-// /// just to demonstrate how that would go
+// // (** [return]: easy, just use Ret *)
+// // let return #s (#c:comm_monoid s) #a (x:a) (post:a -> c.r)
+// //   : eff a (post x) post
+// //   = Ret x
 
-// /// Heaps are usually in a universe higher than the values they store
-// /// Pick it in universe 1
-// assume val heap : Type u#1
+// // (**
+// //  * [bind]: sequential composition works by pushing `g` into the continuation
+// //  * at each node, finally applying it at the terminal `Ret`
+// //  *)
+// // let rec bind #s (#c:comm_monoid s) #a #b (#p:c.r) (#q:a -> c.r) (#r:b -> c.r)
+// //              (f:eff a p q)
+// //              (g: (x:a -> eff b (q x) r))
+// //   : Dv (eff b p r)
+// //   = match f with
+// //     | Ret x -> g x
+// //     | Act act k ->
+// //       Act act (fun x -> bind (k x) g)
+// //     | Par pre0 post0 l
+// //           pre1 post1 r
+// //           k ->
+// //       Par pre0 post0 l pre1 post1 r (fun x0 x1 -> bind (k x0 x1) g)
 
-// /// Assume some monoid of heap assertions
-// assume val hm : comm_monoid heap
-
-// /// For this demo, we'll also assume that this assertions are affine
-// ///  i.e., it's ok to forget some properties of the heap
-// assume val hm_affine (r0 r1:hm.r) (h:heap)
-//   : Lemma (hm.interp (r0 `hm.star` r1) h ==>
-//            hm.interp r0 h)
-
-// /// Here's a ref type
-// assume val ref : Type u#0 -> Type u#0
-
-// /// And two atomic heap assertions
-// assume val ptr_live (r:ref 'a) : hm.r
-// assume val pts_to (r:ref 'a) (x:'a) : hm.r
-
-// /// sel: Selected a reference from a heap, when that ref is live
-// assume val sel (x:ref 'a) (h:heap{hm.interp (ptr_live x) h})
-//   : Tot 'a
-// /// this tells us that sel is frameable
-// assume val sel_ok (x:ref 'a) (h:heap) (frame:hm.r)
-//   : Lemma (hm.interp (ptr_live x `hm.star` frame) h ==>
-//            (hm_affine (ptr_live x) frame h;
-//             let v = sel x h in
-//             hm.interp (pts_to x v `hm.star` frame) h))
+// // (**
+// //  * [par]: Parallel composition
+// //  * Works by just using the `Par` node and `Ret` as its continuation
+// //  **)
+// // let par #s (#c:comm_monoid s)
+// //         #a0 #p0 #q0 (m0:eff a0 p0 q0)
+// //         #a1 #p1 #q1 (m1:eff a1 p1 q1)
+// //  : eff (a0 & a1) (p0 `c.star` p1) (fun (x0, x1) -> q0 x0 `c.star` q1 x1)
+// //  = Par p0 q0 m0
+// //        p1 q1 m1
+// //        #_ #(fun (x0, x1) -> c.star (q0 x0) (q1 x1)) (fun x0 x1 -> Ret (x0, x1))
 
 
-// /// upd: updates a heap at a given reference, when the heap contains it
-// assume val upd (x:ref 'a) (v:'a) (h:heap{hm.interp (ptr_live x) h})
-//   : Tot heap
-// /// and upd is frameable too
-// assume val upd_ok (x:ref 'a) (v:'a) (h:heap) (frame:hm.r)
-//   : Lemma (hm.interp (ptr_live x `hm.star` frame) h ==>
-//            (hm_affine (ptr_live x) frame h;
-//             let h' = upd x v h in
-//             hm.interp (pts_to x v `hm.star` frame) h'))
+// // /// Now for an instantiation of the state with a heap
+// // /// just to demonstrate how that would go
 
-// /// Here's a sample action for dereference
-// let (!) (x:ref 'a)
-//   : eff 'a (ptr_live x) (fun v -> pts_to x v)
-//   = let act : action hm 'a =
-//     {
-//       pre = ptr_live x;
-//       post = pts_to x;
-//       sem = (fun frame h0 ->
-//         hm_affine (ptr_live x) frame h0;
-//         sel_ok x h0 frame;
-//         (| sel x h0, h0 |))
-//     } in
-//     Act act Ret
+// // /// Heaps are usually in a universe higher than the values they store
+// // /// Pick it in universe 1
+// // assume val heap : Type u#1
 
-// /// And a sample action for assignment
-// let (:=) (x:ref 'a) (v:'a)
-//   : eff unit (ptr_live x) (fun _ -> pts_to x v)
-//   = let act : action hm unit =
-//     {
-//       pre = ptr_live x;
-//       post = (fun _ -> pts_to x v);
-//       sem = (fun frame h0 ->
-//         hm_affine (ptr_live x) frame h0;
-//         upd_ok x v h0 frame;
-//         (| (), upd x v h0 |))
-//     } in
-//     Act act Ret
+// // /// Assume some monoid of heap assertions
+// // assume val hm : comm_monoid heap
+
+// // /// For this demo, we'll also assume that this assertions are affine
+// // ///  i.e., it's ok to forget some properties of the heap
+// // assume val hm_affine (r0 r1:hm.r) (h:heap)
+// //   : Lemma (hm.interp (r0 `hm.star` r1) h ==>
+// //            hm.interp r0 h)
+
+// // /// Here's a ref type
+// // assume val ref : Type u#0 -> Type u#0
+
+// // /// And two atomic heap assertions
+// // assume val ptr_live (r:ref 'a) : hm.r
+// // assume val pts_to (r:ref 'a) (x:'a) : hm.r
+
+// // /// sel: Selected a reference from a heap, when that ref is live
+// // assume val sel (x:ref 'a) (h:heap{hm.interp (ptr_live x) h})
+// //   : Tot 'a
+// // /// this tells us that sel is frameable
+// // assume val sel_ok (x:ref 'a) (h:heap) (frame:hm.r)
+// //   : Lemma (hm.interp (ptr_live x `hm.star` frame) h ==>
+// //            (hm_affine (ptr_live x) frame h;
+// //             let v = sel x h in
+// //             hm.interp (pts_to x v `hm.star` frame) h))
+
+
+// // /// upd: updates a heap at a given reference, when the heap contains it
+// // assume val upd (x:ref 'a) (v:'a) (h:heap{hm.interp (ptr_live x) h})
+// //   : Tot heap
+// // /// and upd is frameable too
+// // assume val upd_ok (x:ref 'a) (v:'a) (h:heap) (frame:hm.r)
+// //   : Lemma (hm.interp (ptr_live x `hm.star` frame) h ==>
+// //            (hm_affine (ptr_live x) frame h;
+// //             let h' = upd x v h in
+// //             hm.interp (pts_to x v `hm.star` frame) h'))
+
+// // /// Here's a sample action for dereference
+// // let (!) (x:ref 'a)
+// //   : eff 'a (ptr_live x) (fun v -> pts_to x v)
+// //   = let act : action hm 'a =
+// //     {
+// //       pre = ptr_live x;
+// //       post = pts_to x;
+// //       sem = (fun frame h0 ->
+// //         hm_affine (ptr_live x) frame h0;
+// //         sel_ok x h0 frame;
+// //         (| sel x h0, h0 |))
+// //     } in
+// //     Act act Ret
+
+// // /// And a sample action for assignment
+// // let (:=) (x:ref 'a) (v:'a)
+// //   : eff unit (ptr_live x) (fun _ -> pts_to x v)
+// //   = let act : action hm unit =
+// //     {
+// //       pre = ptr_live x;
+// //       post = (fun _ -> pts_to x v);
+// //       sem = (fun frame h0 ->
+// //         hm_affine (ptr_live x) frame h0;
+// //         upd_ok x v h0 frame;
+// //         (| (), upd x v h0 |))
+// //     } in
+// //     Act act Ret
